XXX Try (and fail) to adapt saved_pred for our needs
It seems I have a mismatch between different sorts of functions, maybe
normal functions vs ofe_mor. That's hard to see when looking at pretty-printed
types, it might be more visible when printing rawer terms (disabling notations
and implicits).

theories/experiments.v
@@ -76,6 +76,95 @@ Section Sec.
   (* From iris Require Import algebra.ofe. *)
   (* Check savedEnvD. *)
   (* Alternative to savedPredG *)
-  Canonical Structure listVlC := leibnizC (list vl).
-  Definition savedEnvDG := (savedAnythingG Σ (listVlC -n> vlC -c> ▶ ∙)%CF).
+  Notation savedEnvDG := (savedAnythingG Σ (listVlC -c> vlC -c> ▶ ∙)%CF).
+  Notation savedEnvDΣ := (savedAnythingΣ (listVlC -c> vlC -c> ▶ ∙)).
+
+  (* Notation savedEnvDG := (savedAnythingG Σ (listVlC -c> vlC -c> ▶ ∙)). *)
+  (* Notation savedEnvDΣ := (savedAnythingΣ (listVlC -c> vlC -c> ▶ ∙)). *)
+  (* Print saved_anything_own. *)
+  (* Print savedAnythingG. *)
+  (* Print cFunctor. *)
+  Print savedPredG.
+  Print saved_pred_own.
+
+  Print saved_anything_own.
+  Context `{savedEnvDG}.
+  Program Definition saved_envDG_own (γ : gname) (Φ : listVlC -n> vlC -n> iProp Σ): iProp Σ :=
+    saved_anything_own (F := listVlC -c> vlC -c> ▶ ∙) γ (λ ρ, λne v, Next (Φ ρ v)).
+
+  Instance saved_envDG_own_contractive γ:
+    Contractive
+                (saved_envDG_own γ: (listVlC -n> vlC -n> iProp Σ) → iProp Σ).
+  Proof.
+    solve_proper_core ltac:(fun _ =>
+                    first [ intros ? ?; progress simpl | by auto | f_contractive | f_equiv ]).
+
+    (* solve_proper_prepare. *)
+
+    (* repeat first [eassumption | first [ intros ? ?; progress simpl | by auto | f_contractive | f_equiv ]]. *)
+    (* cbn in H0. *)
+    (* solve [apply H0]. *)
+    (* Restart. *)
+    (* (* Summarizes to: *) *)
+    (* solve_proper_core ltac:(fun _ => *)
+    (*                 first [ intros ? ?; progress simpl | by auto | f_contractive | f_equiv | apply H0 ]). *)
+    (* (* But that is really fragile.*) *)
+  Qed.
+
+  Lemma saved_envDG_alloc_strong (G : gset gname) (Φ : listVlC -n> vlC -n> iProp Σ) :
+    (|==> ∃ γ, ⌜γ ∉ G⌝ ∧ saved_envDG_own γ Φ)%I.
+  Proof. iApply saved_anything_alloc_strong. Qed.
+
+  Lemma saved_envDG_alloc (Φ : listVlC -n> vlC -n> iProp Σ) :
+    (|==> ∃ γ, saved_envDG_own γ Φ)%I.
+  Proof. iApply saved_anything_alloc. Qed.
+
+  (* We put the `x` on the outside to make this lemma easier to apply. *)
+  Lemma saved_envDG_agree1 `{savedPredG Σ A} γ Φ Ψ x :
+    saved_envDG_own γ Φ -∗ saved_envDG_own γ Ψ -∗ ▷ (Φ x ≡ Ψ x).
+    unfold saved_envDG_own. iIntros "#HΦ #HΨ".
+    Import uPred.
+    iApply later_equivI.
+    Check @saved_anything_agree.
+    Eval hnf in (listVlC -c> vlC -c> ▶ iProp Σ)%CF.
+    iDestruct (saved_anything_agree (F := listVlC -c> vlC -c> ▶ ∙) with "HΦ HΨ") as "Heq".
+    simpl.
+
+    Check @ofe_fun_equivI.
+    iDestruct (@ofe_fun_equivI _ (listVlC) (λ _, vlC -n> laterC (iProp Σ)) (λ ρ, λne v, Next (Φ ρ v)) (λ ρ, λne v, Next (Ψ ρ v))) as "[Heq1 _]".
+    Fail iSpecialize ("Heq1" with "Heq").
+    Abort.
+  (* (*   by iDestruct ("Heq1" with "Heq") as "?". *) *)
+
+  (* (*   simpl. *) *)
+  (* (*   Unset Printing Notations. *) *)
+  (* (*   Set Printing Implicit. *) *)
+  (* (*   simpl in *. *) *)
+  (* (*   iDestruct ("Heq1" with "Heq") as "?". *) *)
+  (* (*   iApply "Heq1". *) *)
+
+  (* (*  "Heq" : (λ (ρ : listVlC) (v : vlC), Next (Φ ρ v)) *) *)
+  (* (*         ≡ (λ (ρ : listVlC) (v : vlC), Next (Ψ ρ v)) *) *)
+  (* (*   iDestruct (ofe_fun_equivI with "Heq"). as "?". *) *)
+  (* (*   by iDestruct (ofe_fun_equivI with "Heq") as "?". *) *)
+  (* (* Qed. *) *)
+
+  (* Lemma saved_envDG_agree `{savedPredG Σ A} γ Φ Ψ x y : *)
+  (*   saved_envDG_own γ Φ -∗ saved_envDG_own γ Ψ -∗ ▷ (Φ x y ≡ Ψ x y). *)
+  (* Proof. *)
+  (*   unfold saved_envDG_own. iIntros "#HΦ #HΨ /=". *)
+  (*   Import uPred. *)
+  (*   iApply later_equivI. *)
+  (*   Check @saved_anything_agree. *)
+  (*   Eval hnf in (listVlC -c> vlC -c> ▶ iProp Σ)%CF. *)
+  (*   iDestruct (saved_anything_agree (F := listVlC -c> vlC -c> ▶ ∙) with "HΦ HΨ") as "Heq". *)
+  (*   Check @ofe_fun_equivI. *)
+  (*   epose proof (@ofe_fun_equivI _ (listVlC) (λ _, vlC -n> laterC (iProp Σ)) (λne ρ, λne v, CofeMor Next (Φ ρ v)) (λ ρ, λne v, Next (Ψ ρ v))). *)
+  (*   iDestruct (H0 with "Heq") as "?". *)
+
+  (*  "Heq" : (λ (ρ : listVlC) (v : vlC), Next (Φ ρ v)) *)
+  (*         ≡ (λ (ρ : listVlC) (v : vlC), Next (Ψ ρ v)) *)
+  (*   iDestruct (ofe_fun_equivI with "Heq"). as "?". *)
+  (*   by iDestruct (ofe_fun_equivI with "Heq") as "?". *)
+  (* Qed. *)
 End Sec.
